% \begin{figure} \label{fig:upsilon}
% \centerline{\xymatrix{
% A_0 \ar@/^5pc/[r]^{f_0} 
% \ar@/^2pc/[r]^{\big\Downarrow \phi_1}_{f_1} 
% \ar@/_2pc/[r]^{\substack{\vdots\\ f_n}}
% \ar@/_5pc/[rrr]_{id}^{\substack{\alpha \\ \\ \\ \\ }}
% & A_1 \ar@/^5pc/[r]^{g_0} 
% \ar@/^2pc/[r]^{\big\Downarrow \psi_1}_{g_1} 
% \ar@/_2pc/[r]^{\substack{\vdots\\ g_m}}
% & A_2 \ar@/^5pc/[r]^{h_0} 
% \ar@/^2pc/[r]^{\big\Downarrow \theta_1}_{h_1} 
% \ar@/_2pc/[r]^{\substack{\vdots\\ h_p}}
% & A_0
% }
% $\overset{[d_0^* \Upsilon, \mathcal{B}]}\longrightarrow$
% \xymatrix{
% A_0 \ar@/^5pc/[r]^{f_0} 
% \ar@/^2pc/[r]^{\big\Downarrow \phi_1}_{f_1} 
% \ar@/_2pc/[r]^{\substack{\vdots\\ f_n}}
% \ar@/_5pc/[rrr]_{id}^{\substack{\alpha \\ \\ \\ \\ }}
% & A_1 \ar@/^5pc/[r]^{g_0} 
% \ar@/^2pc/[r]^{\big\Downarrow \psi_1}_{g_1} 
% \ar@/_2pc/[r]^{\substack{\vdots\\ g_m}}
% & A_2 \ar@/^5pc/[r]^{h_0} 
% \ar@/^2pc/[r]^{\big\Downarrow \theta_1}_{h_1} 
% \ar@/_2pc/[r]^{\substack{\vdots\\ h_p}}
% & A_0
% }}
% \caption{A picture of the domain and target of $[d_0^* \Upsilon, \mathcal{B}]$}
% \end{figure}

\begin{prop}
\label{prop:c5}
Let $\Upsilon$ and $\mathcal{B}$ be as 
defined in the previous propositions. 
Then, $[\Upsilon, \mathcal{B}] := 
\Upsilon_{A_1\bullet A_2, A_0} 
\mathcal{B}_{A_0,A_1,A_2} - 
\mathcal{B}_{A_2, A_0, A_1} 
\Upsilon_{A_0 \bullet A_1, A_2} = 0$. 
(Note that $[\Upsilon, \mathcal{B}]$ is 
a map from $C(A_0 \to A_1 \to A_2 \to A_0)$ 
to itself.)
\end{prop}
%
\begin{proof}
We show the proposition by direct computation. 
Since all of the maps are maps of cofree 
comodules, we only need to check that 
$\pi_1([\Upsilon, \mathcal{B}]) = 0$ where 
$\pi_1$ denotes projection of the comodule 
onto cogenerators. We check this directly.
%
\begin{equation*}
\begin{aligned}
&\phantom{{}={}}
\pi_1 \circ \Upsilon_{A_1\bullet A_2, A_0} 
  \mathcal{B}_{A_0,A_1,A_2} 
  (\vec{\phi} | \vec{\psi} | \vec{\theta} | \alpha ) \\
&= 
\sum \limits_{\substack{
  I_1I_2 = \{1,\smdots,n\}\\
  J_1J_2 = \{1,\smdots,m\}\\
  K_1K_2 = \{1,\smdots,p\}\\
  \textrm{as ordered sets}}}
\epsilon_{I_1,J_1,K_1}\cdot
\upsilon_{|K_1| \leq * \leq |K_1|+|J_1|, |I_1|} (
   \vec{\psi}_{J_1} \bullet \vec{\theta}_{K_1} | 
   \vec{\phi}_{I_1} | 
   \mathcal{B}_{|I_2|, |J_2|, |K_2|} (
   \vec{\phi}_{I_2} | \vec{\psi}_{J_2} | \vec{\theta}_{K_2} | \alpha)) \\
&= 
\sum \limits_{\substack{
  I_1I_2 = \{1,\smdots,n\}\\
  J_1J_2 = \{1,\smdots,m\}\\
  K_1K_2 = \{1,\smdots,p\}\\
  \textrm{as ordered sets}}}
\epsilon_{I_1,J_1,K_1}\cdot
\eta_{\mathfrak{a}_1, \mathfrak{a}_2} \cdot
\upsilon_{|K_1| \leq * \leq |K_1|+|J_1|, |I_1|} (
   \vec{\psi}_{J_1} \bullet \vec{\theta}_{K_1} | 
   \vec{\phi}_{I_1} |
   1 \otimes \lambda(\vec{\phi}_{I_2})[
     \lambda(\vec{\theta}_{K_2}) \lambda(\vec{\psi}_{J_2}) 
     \lambda(\vec{\phi}_{I_3}) 
     \mathfrak{a}_2, a_0, \mathfrak{a}_1] \\
&= 
\sum \limits_{\substack{
  I_1I_2 = \{1,\smdots,n\}\\
  J_1J_2 = \{1,\smdots,m\}\\
  K_1K_2 = \{1,\smdots,p\}\\
  \textrm{as ordered sets}}}
\epsilon_{I_1,J_1,K_1}\cdot
\eta_{\mathfrak{a}_1, \mathfrak{a}_2} \cdot
1 \otimes \lambda(\vec{\theta}_{K_1}) \lambda(\vec{\psi}_{J_1}) 
  \lambda(\vec{\phi}_{I_1})[
     \lambda(\vec{\theta}_{K_2}) \lambda(\vec{\psi}_{J_2}) 
     \lambda(\vec{\phi}_{I_2})
     \mathfrak{a}_2, a_0, \mathfrak{a}_1]    
\end{aligned}
\end{equation*}
%
\begin{align*}
& \phantom{{}={}}
\pi_1 \circ \mathcal{B}_{A_2, A_0, A_1} 
  \Upsilon_{A_0 \bullet A_1, A_2} 
  (\vec{\phi} | \vec{\psi} | \vec{\theta} | \alpha ) \\
&= 
\sum \limits_{\substack{
  I_1I_2 = \{1,\smdots,n\}\\
  J_1J_2 = \{1,\smdots,m\}\\
  K_1K_2 = \{1,\smdots,p\}\\
  \textrm{as ordered sets}}}
\epsilon_{I_1,J_1,K_1}\cdot
B_{|K_1|, |I_1|, |J_1|} 
   (\vec{\theta}_{K_1} | \vec{\phi}_{I_1} | \vec{\psi}_{J_1} | 
   \upsilon_{|J_2| \leq * \leq |I_2|+|J_2|, |K_2|} 
   (\vec{\phi}_{I_2} \bullet \vec{\psi}_{J_2} | \vec{\theta}_{K_2} | \alpha)) \\
&= 
\sum \limits_{\substack{
  I_1I_2 = \{1,\smdots,n\}\\
  J_1J_2 = \{1,\smdots,m\}\\
  K_1K_2 = \{1,\smdots,p\}\\
  \textrm{as ordered sets}}}
\epsilon_{I_1,J_1,K_1}\cdot
\eta_{\mathfrak{a}_1, \mathfrak{a}_2} \cdot
1 \otimes \lambda(\vec{\theta}_{K_1}) \lambda(\vec{\psi}_{J_1}) 
  \lambda(\vec{\phi}_{I_1})[
     \lambda(\vec{\theta}_{K_2}) \lambda(\vec{\psi}_{J_2}) 
     \lambda(\vec{\phi}_{I_2})
     \mathfrak{a}_2, a_0, \mathfrak{a}_1]  
\end{align*}
where $\epsilon_{I_1,J_1,K_1} = 
(-1)^{(\sum \limits_{r \in I_2}|\phi_r|+1)
  ((\sum \limits_{s \in J_1}|\psi_s|+1) + 
  (\sum \limits_{t \in K_1}|\theta_t|+1)) + 
  (\sum \limits_{s \in J_2}|\psi_s|+1)
  (\sum \limits_{t \in K_1}|\theta_t|+1)}$
and $\eta_{\mathfrak{a}_1, \mathfrak{a}_2} = 
(-1)^{|\mathfrak{a}_1|(|\mathfrak{a}_1+ 
\mathfrak{a}_2|)}$.
It's clear that $\pi_1([\Upsilon, \mathcal{B}]) = 0$.
\end{proof}