% \begin{figure} \label{fig:upsilon}
% \centerline{\xymatrix{
% A_0 \ar@/^5pc/[r]^{f_0} 
% \ar@/^2pc/[r]^{\big\Downarrow \phi_1}_{f_1} 
% \ar@/_2pc/[r]^{\substack{\vdots\\ f_n}}
% \ar@/_5pc/[rrr]_{id}^{\substack{\alpha \\ \\ \\ \\ }}
% & A_1 \ar@/^5pc/[r]^{g_0} 
% \ar@/^2pc/[r]^{\big\Downarrow \psi_1}_{g_1} 
% \ar@/_2pc/[r]^{\substack{\vdots\\ g_m}}
% & A_2 \ar@/^5pc/[r]^{h_0} 
% \ar@/^2pc/[r]^{\big\Downarrow \theta_1}_{h_1} 
% \ar@/_2pc/[r]^{\substack{\vdots\\ h_p}}
% & A_0
% }
% $\overset{\mathcal{B}}\longrightarrow$
% \xymatrix{
% A_2 \ar@/^5pc/[r]^{h_0} 
% \ar@/^2pc/[r]^{\big\Downarrow \theta_1}_{h_1} 
% \ar@/_2pc/[r]^{\substack{\vdots\\ h_p}}
% \ar@/_5pc/[rrr]_{id}^{\substack{\alpha \\ \\ \\ \\ }}
% & A_0 \ar@/^5pc/[r]^{f_0} 
% \ar@/^2pc/[r]^{\big\Downarrow \phi_1}_{f_1} 
% \ar@/_2pc/[r]^{\substack{\vdots\\ f_n}}
% & A_1 \ar@/^5pc/[r]^{g_0} 
% \ar@/^2pc/[r]^{\big\Downarrow \psi_1}_{g_1} 
% \ar@/_2pc/[r]^{\substack{\vdots\\ g_m}}
% & A_2
% }}
% \caption{A picture of the domain and target of $\mathcal{B}$}
% \end{figure}
%
\begin{prop} \label{prop:c4}
Let 
$$
\mathcal{B}: C(A_0 \to A_1 \to A_2 \to A_0)
\to \hat{\tau}_2^{*2}C(A_1 \to A_2 \to A_0 \to A_1)
$$ 
be a map of comodules over 
$B(A_0 \to A_1 \to A_2 \to A_0)$ 
determined by the following maps to 
cogenerators:
\begin{align*}
\mathcal{B}^{f_0, g_0,h_0}: 
  C(A_0 \to A_1 \to A_0)(h_0g_0f_0) 
&\to
\hat{\tau}_2^{*2}C(A_1 \to A_2 \to A_0 \to A_1)
  (f_0h_0g_0)\\
&\xrightarrow[cogenerators]{\textrm{project onto}}
C_{-\bullet}(A_1, _{f_0h_0g_0}{A_1}_{id})\\
\mathcal{B}_{n, m, p} (\vec{\phi} | \vec{\psi} | \vec{\theta} | \alpha) 
= & \sum_{\substack{I_1I_2 = \{1,2,\cdots,n\} \\
                          \textrm{as ordered sets}}}
  1 \otimes \lambda(\vec{\phi}_{I_1})\big( \lambda(\vec{\theta}) \lambda(\vec{\psi}) \lambda(\vec{\phi}_{I_2})
  \mathfrak{a}_2 \otimes a_0 \otimes \mathfrak{a}_1 \big)               
\end{align*}
Then, 
\begin{equation} \label{eq:prop4}
D(\mathcal{B}) = 
  \Upsilon_{A_2\bullet A_0, A_1} \circ
  \Upsilon_{A_0\bullet A_1, A_2} 
   - \Upsilon_{A_0, A_1\bullet A_2}.
\end{equation}
\end{prop}

\begin{proof}
We will show that Equation \ref{eq:prop4} 
holds by direct computation. Since all of 
the maps are maps of cofree comodules, we 
only need to check that $\pi_1($
Equation \ref{eq:prop4}$)$ holds where 
$\pi_1$ denotes projection of the comodule 
onto cogenerators. More explicitly, we 
want to check that
\begin{equation} \label{eq:prop4_expand}
\begin{aligned}
%hochschild cochain delta
\mathcal{B}_{n, m, p} ( \tilde{\delta}(\vec{\phi}) | \vec{\psi} | \vec{\theta} | \alpha ) \; + 
\mathcal{B}_{n, m, p} ( \vec{\phi} | \tilde{\delta}(\vec{\psi}) | \vec{\theta} | \alpha ) \; + 
\mathcal{B}_{n, m, p} ( \vec{\phi} | \vec{\psi} | \tilde{\delta}(\vec{\theta}) | \alpha ) \; + \\
%cochain b prime
\mathcal{B}_{n-1, m, p} ( b^\prime(\vec{\phi}) | \vec{\psi} | \vec{\theta} | \alpha ) \; + 
\mathcal{B}_{n, m-1, p} ( \vec{\phi} | b^\prime(\vec{\psi}) | \vec{\theta} | \alpha ) \; + 
\mathcal{B}_{n, m, p-1} ( \vec{\phi} | \vec{\psi} | b^\prime(\vec{\theta}) | \alpha ) \; + \\
%chain b
\mathcal{B}_{n, m, p} ( \vec{\phi} | \vec{\psi} | \vec{\theta} | b(\alpha) ) \; + 
b \circ \mathcal{B}_{n, m, p} ( \vec{\phi} | \vec{\psi} | \vec{\theta} | \alpha ) \; + \\
%twist before
 \mathcal{B}_{|I_1|, |J_1|, p-1}(\vec{\phi}_{I_1} | \vec{\psi}_{J_1} | \vec{\theta}_{\{1,\cdots, p-1\}} |
     \theta_{p} \{\vec{\psi}_{J_2}\} \{\vec{\phi}_{I_2}\} \cdot \alpha ) \; + \\
 \mathcal{B}_{|I_1|, m-1, p}(\vec{\phi}_{I_1} | \vec{\psi}_{\{1,\cdots, m-1\}} | \vec{\theta} |
     \psi_{m} \{\vec{\phi}_{I_2}\}\cdot \alpha ) \; + 
\mathcal{B}_{n-1, m, p}(\vec{\phi}_{\{1,\cdots, n-1\}} |\vec{\psi}_{m} | \vec{\theta} | 
     \phi_{n} \cdot \alpha) \; + \\
%twist after
\phi_1 \{\vec{\theta}_{K_1}\} \{\vec{\psi}_{J_1}\} \cdot
     \mathcal{B}_{n-1, |J_2|, |K_2|}
     (\vec{\phi}_{\{2,\cdots,n\}} | \vec{\psi}_{J_2} | \vec{\theta}_{K_2} | \alpha) \; + \\
\theta_1 \{\vec{\psi}_{J_1}\} \cdot
     \mathcal{B}_{n, |J_2|, p-1}
     (\vec{\phi} | \vec{\psi}_{J_2} | \vec{\theta}_{\{2,\cdots,p\}} | \alpha) \; +
\psi_1 \cdot
     \mathcal{B}_{n, m-1, p}
     (\vec{\phi} | \vec{\psi}_{\{2,\cdots,m\}} | \vec{\theta} | \alpha) \; + \\
%prop4
\upsilon_{n, p \leq * \leq m+p}(\vec{\phi} | \vec{\psi} \bullet \vec{\theta} | \alpha ) \; + \\
\upsilon_{|I_1| \leq * \leq |I_1| + |K_1|,|J_1|}(\vec{\theta}_{K_1} \bullet \vec{\phi}_{I_1}, \vec{\psi}_{J_1}, 
    \upsilon_{|J_2| \leq * \leq |I_2| + |J_2|,|K_2|}(\vec{\phi}_{I_2} \bullet \vec{\psi}_{J_2} | \vec{\theta}_{K_2} | \alpha )) \\
%
=0.
\end{aligned}
\end{equation}
In Equation \ref{eq:prop4_expand} above, 
we call the terms in rows 1-3 the 
``standard terms'' in the computation of 
$D(\mathcal{B})$, and the terms in rows 
4-7 the ``extra terms'' in the computation 
of $D(\mathcal{B})$. The terms in rows 8-9 
are $\pi_1$ of the righthand side of Equation 
\ref{eq:prop4}; we will call these the 
``8$^{th}$- and 9$^{th}$-row terms''.

We compute the sum of the standard terms. 
In the chart below, the leftmost column lists 
the expressions that don't cancel in the sum 
of the standard terms, the middle column gives 
the standard term from which the expression comes, 
and the rightmost column gives the term that 
cancels the expression. 
\newpage
\begin{landscape}
\begin{center}
  \begin{tabular}{ p{3.25in} | p{1.75in} | p{2.75in} }
    \hline
    Expression & Comes from Standard Term & Cancelling Term \\ \hline
    %
    % twist before
    $1 \otimes \lambda(\vec{\phi}_{I_1}) [
    \lambda(\vec{\theta}_{\{1,\cdots,p-1\}}
    \lambda(\vec{\psi}_{J_1})
    \lambda(\vec{\phi}_{I_2})
    \mathfrak{a}_2 \otimes 
    \theta_p(\lambda(\vec{\psi}_{J_2}) \lambda(\vec{\phi}_{I_3}) \mathfrak{a}_3) \cdot a_0 \otimes
    \mathfrak{a}_1 ]$ & 
    $b \circ \mathcal{B}_{n,m,p} (\vec{\phi} | \vec{\psi} | \vec{\theta} | \alpha)$ & 
    $\mathcal{B}_{|I_1|, |J_1|, p-1}(\vec{\phi}_{I_1} | \vec{\psi}_{J_1} | \vec{\theta}_{\{1,\cdots, p-1\}} |
     \theta_{p} \{\vec{\psi}_{J_2}\} \{\vec{\phi}_{I_2}\} \cdot \alpha )$ \\ \hline

    $1 \otimes \lambda(\vec{\phi}_{I_1}) [
    \lambda(\vec{\theta}
    \lambda(\vec{\psi}_{\{1,\cdots,m-1\}})
    \lambda(\vec{\phi}_{I_2})
    \mathfrak{a}_2 \otimes 
    \psi_m(\lambda(\vec{\phi}_{I_3}) \mathfrak{a}_3) \cdot a_0 \otimes
    \mathfrak{a}_1 ]$ & 
    $b \circ \mathcal{B}_{n,m,p} (\vec{\phi} | \vec{\psi} | \vec{\theta} | \alpha)$ & 
    $\mathcal{B}_{|I_1|, m-1, p}(\vec{\phi}_{I_1} | \vec{\psi}_{\{1,\cdots, m-1\}} | \vec{\theta} |
     \psi_m \{\vec{\phi}_{I_2}\} \cdot \alpha )$ \\ \hline

    $1 \otimes \lambda(\vec{\phi}_{I_1}) [
    \lambda(\vec{\theta}
    \lambda(\vec{\psi}
    \lambda(\vec{\phi}_{\{1,\cdots,n-1\}})
    \mathfrak{a}_2 \otimes 
    \psi_n(\mathfrak{a}_3) \cdot a_0 \otimes
    \mathfrak{a}_1 ]$ & 
    $b \circ \mathcal{B}_{n,m,p} (\vec{\phi} | \vec{\psi} | \vec{\theta} | \alpha)$ & 
    $\mathcal{B}_{n-1, m, p}(\vec{\phi}_{\{1,\cdots, n-1\}} | \vec{\psi} | \vec{\theta} |
     \phi_n \cdot \alpha )$ \\ \hline
    %
    %twist after
    $\phi_1(\lambda(\vec{\theta}_{K_1}) \lambda(\vec{\psi}_{J_1}) \lambda(\vec{\phi}_{I_2}) \mathfrak{a}_2)
    \otimes \lambda(\vec{\phi}_{I_1\backslash 1})[
    \lambda(\vec{\theta}_{K_2}) \lambda(\vec{\psi}_{J_3}) \lambda(\vec{\phi}_{I_3}) \mathfrak{a}_3
    \otimes a_0 \otimes \mathfrak{a}_1]$ &
    $b \circ \mathcal{B}_{n,m,p} (\vec{\phi} | \vec{\psi} | \vec{\theta} | \alpha)$ & 
    $\phi_1 \{\vec{\theta}_{K_1}\} \{\vec{\psi}_{J_1}\} \cdot
     \mathcal{B}_{n-1, |J_2|, |K_2|}
     (\vec{\phi}_{\{2,\cdots,n\}} | \vec{\psi}_{J_2} | \vec{\theta}_{K_2} | \alpha)$ \\ \hline

    $f_0\theta_1( \lambda(\vec{\psi}_{J_1}) \lambda(\vec{\phi}_{I_2}) \mathfrak{a}_2)
    \otimes \lambda(\vec{\phi}_{I_1})[
    \lambda(\vec{\theta}_{\{2,\cdots,p\}}) \lambda(\vec{\psi}_{J_2}) \lambda(\vec{\phi}_{I_3}) \mathfrak{a}_3
    \otimes a_0 \otimes \mathfrak{a}_1]$ &
    $b \circ \mathcal{B}_{n,m,p} (\vec{\phi} | \vec{\psi} | \vec{\theta} | \alpha)$ & 
    $\theta_1 \{\vec{\psi}_{J_1}\} \cdot
     \mathcal{B}_{n, |J_2|, p-1}
     (\vec{\phi} | \vec{\psi}_{J_2} | \vec{\theta}_{\{2,\cdots,p\}} | \alpha)$ \\ \hline

    $f_0h_0\psi_1( \lambda(\vec{\phi}_{I_2}) \mathfrak{a}_2)
    \otimes \lambda(\vec{\phi}_{I_1})[
    \lambda(\vec{\theta}) \lambda(\vec{\psi}_{\{2,\cdots,m\}}) \lambda(\vec{\phi}_{I_3}) \mathfrak{a}_3
    \otimes a_0 \otimes \mathfrak{a}_1]$ &
    $b \circ \mathcal{B}_{n,m,p} (\vec{\phi} | \vec{\psi} | \vec{\theta} | \alpha)$ & 
    $\psi_1 \cdot
     \mathcal{B}_{n, m-1, p}
     (\vec{\phi} | \vec{\psi}_{\{2,\cdots,m\}} | \vec{\theta} | \alpha)$ \\ \hline

    %wrap around
    $f_0h_0g_0 \phi_{i_1} ( \lambda(\vec{\theta}_{K_2}) \lambda(\vec{\psi}_{J_2}) \lambda(\vec{\phi}_{I_3})
       \mathfrak{a}_3 \otimes a_0 \otimes \mathfrak{a}_1) \otimes
       \lambda(\vec{\phi}_{I_1}) \lambda(\vec{\theta}_{K_1}) \lambda(\vec{\psi}_{J_1}) 
       \lambda(\vec{\phi}_{I_2 \backslash i_1}) \mathfrak{a}_2$ &
    $b \circ \mathcal{B}_{n,m,p} (\vec{\phi} | \vec{\psi} | \vec{\theta} | \alpha)$ & 
    9$^{th}$ row \\ \hline

    $f_0h_0g_0f_{i_1}a_0 \otimes \lambda(\vec{\phi}_{I_1}) \lambda(\vec{\theta}) 
       \lambda(\vec{\psi}_{J_1}) \lambda(\vec{\phi}_{I_2}) \mathfrak{a}_1$ &
    $b \circ \mathcal{B}_{n,m,p} (\vec{\phi} | \vec{\psi} | \vec{\theta} | \alpha)$ & 
    9$^{th}$ row \\ \hline

    $\phi_1( \lambda(\vec{\phi}_{I_1}) \lambda(\vec{\theta}) 
       \lambda(\vec{\psi}_{J_1}) \lambda(\vec{\phi}_{I_2}) \mathfrak{a}_3, a_0, \mathfrak{a}_1 ) \otimes
       \lambda(\vec{\phi}_{I_1 \backslash 1}) \mathfrak{a}_2$ &
    $b \circ \mathcal{B}_{n,m,p} (\vec{\phi} | \vec{\psi} | \vec{\theta} | \alpha)$ & 
    8$^{th}$ row \\ \hline

  \end{tabular}
\end{center}
\end{landscape}

\newpage
\begin{landscape}

Now, we compute the remaining terms from the ninth row. In the chart below, the left column lists the remaining expressions that don't cancel in the ninth row, and the right column gives the extra term that cancels the expression. 

\begin{center}
  \begin{tabular}{ p{6.25in} | p{2.5in} }
    \hline
    Expression from ninth Row & Cancels with Extra Term \\ \hline
    %twist after
    $\phi_1(\lambda(\vec{\theta}_{K_1}) \lambda(\vec{\psi}_{J_1}) \lambda(\vec{\phi}_{I_2}) [
      \lambda(\vec{\theta}_{K_3}) \lambda(\vec{\psi}_{J_4}) \lambda(\vec{\phi}_{I_5})
      \mathfrak{a}_3, a_0, \mathfrak{a}_1])
      \otimes \lambda(\vec{\phi}_{I_1\backslash 1}) \lambda(\vec{\theta}_{K_2}) 
      \lambda(\vec{\psi}_{J_3}) \lambda(\vec{\phi}_{I_4}) \mathfrak{a}_2$ &
    $\phi_1 \{\vec{\theta}_{K_1}\} \{\vec{\psi}_{J_1}\} \cdot
     \mathcal{B}_{n-1, |J_2|, |K_2|}
     (\vec{\phi}_{\{2,\cdots,n\}} | \vec{\psi}_{J_2} | \vec{\theta}_{K_2} | \alpha)$ \\ \hline

    $f_0\theta_1( \lambda(\vec{\psi}_{J_1}) \lambda(\vec{\phi}_{I_2}) [
      \lambda(\vec{\theta}_{K_2}) \lambda(\vec{\psi}_{J_3}) \lambda(\vec{\phi}_{I_4})
      \mathfrak{a}_3, a_0, \mathfrak{a}_1])
      \otimes \lambda(\vec{\phi}_{I_1}) \lambda(\vec{\theta}_{K_1 \backslash 1}) 
      \lambda(\vec{\psi}_{J_2}) \lambda(\vec{\phi}_{I_3}) \mathfrak{a}_2$ &
    $\theta_1 \{\vec{\psi}_{J_1}\} \cdot
     \mathcal{B}_{n, |J_2|, p-1}
     (\vec{\phi} | \vec{\psi}_{J_2} | \vec{\theta}_{\{2,\cdots,p\}} | \alpha)$ \\ \hline

    $f_0h_0\psi_1( \lambda(\vec{\phi}_{I_2}) [
      \lambda(\vec{\theta}_{K_2}) \lambda(\vec{\psi}_{J_2}) \lambda(\vec{\phi}_{I_4})
      \mathfrak{a}_3, a_0, \mathfrak{a}_1])
      \otimes \lambda(\vec{\phi}_{I_1}) \lambda(\vec{\theta}_{K_1}) 
      \lambda(\vec{\psi}_{J_1 \backslash 1}) \lambda(\vec{\phi}_{I_3}) \mathfrak{a}_2$ & 
    $\psi_1 \cdot
     \mathcal{B}_{n, m-1, p}
     (\vec{\phi} | \vec{\psi}_{\{2,\cdots,m\}} | \vec{\theta} | \alpha)$ \\ \hline

    \hline
  \end{tabular}
\end{center}
\end{landscape}

All of the terms in the table describing the expansion of Equation \ref{eq:prop4_expand} cancel, so we're done.
\end{proof}