\section{Homotopies}
Here, we will show that the maps 
of dg comodules given in Section 
\ref{sec:shriek_maps} satisfy the 
relations in $\Lambda$ (Equation 
\ref{eqn:cyclic_relations}) up to 
homotopy. More precisely, we will 
show that
\begin{subequations}\label{eq:strict}
\begin{align}
\begin{split}\label{eq:strict_1}
\hat{\delta}_{j,n}^*(\delta_{i,n-1!}) \circ \delta_{j,n!} 
&= 
\hat{\delta}_{i,n}^*(\delta_{j-1,n-1!}) \circ \delta_{i,n!} 
  \quad 0 \leq i < j \leq n-1 \\
\hat{\sigma}_{j,n}^*(\sigma_{i,n+1!}) \circ \sigma_{j,n!} 
&= 
\hat{\sigma}_{i,n}^*(\sigma_{j+1,n+1!}) \circ \sigma_{i,n!}
  \quad 0 \leq i \leq j \leq n \\
\hat{\sigma}_{i,n}^*(\delta_{j,n+1!}) \circ \sigma_{i,n!} 
&= 
  \begin{cases}
    \hat{\delta}_{j-1,n}^*(\sigma_{i,n-1!}) \circ \delta_{j-1,n!} 
      & 0 \leq i < j \leq n\\
    id & j = i, i-1\\
    \hat{\delta}_{j,n}^*(\sigma_{i-1,n-1!}) \circ \delta_{j,n!} 
      & \quad 0 \leq j < i-1 \leq n-1
   \end{cases}
\end{split}\\
\begin{split}\label{eq:strict_2}
\hat{\sigma}_{i,n}^*(\tau_{n+1!}) \circ \sigma_{i,n!} 
&= 
\hat{\tau}_n^*(\sigma_{i+1,n!}) \circ \tau_{n!}
  \quad 0 \leq i \leq n-1\\
\hat{\delta}_{j,n}^*(\tau_{n-1!}) \circ \delta_{j,n!} 
&= 
\hat{\tau}_n^*(\delta_{j+1,n!}) \circ \tau_{n!}
  \quad 0 \leq j \leq n-1
\end{split}\\
\begin{split}\label{eq:strict_3}
(\widehat{\tau_{1}\sigma_{0,0}})^*
  (\delta_{0,1!}) \circ
  \hat{\sigma}_{0,0}^*(\tau_{1!}) \circ 
  \sigma_{0,0!}
= id
\end{split} 
\end{align}
\end{subequations}
and 
\begin{subequations} \label{eq:weak}
\begin{equation} \label{eq:weak_delta}
\hat{\tau}_n^{*2}(\delta_{0,n!}) \circ 
  \hat{\tau}_n^*(\tau_{n!}) \circ \tau_{n!} 
\simeq 
\hat{\delta}_{n-1,n}^*(\tau_{n-1!}) \circ \delta_{n-1,n!}
\end{equation}
\begin{equation} \label{eq:weak_tau}
\hat{\tau}_n^{*n}(\tau_{n!}) \circ \smdots 
  \circ \hat{\tau}_n^*(\tau_{n!}) \circ \tau_{n!}
\simeq id
\end{equation}
\begin{equation} \label{eq:weak_sigma}
\hat{\sigma}_{n,n}^*(\tau_{n+1!}) \circ \sigma_{n,n!}
\simeq
(\widehat{\tau_{n+1}^n\sigma_{0,n}\tau_{n}})^*(\tau_{n+1!})
  \circ \smdots \circ 
  (\widehat{\tau_{n+1}\sigma_{0,n}\tau_{n}})^*(\tau_{n+1!}) \circ
  (\widehat{\sigma_{0,n}\tau_{n}})^*(\tau_{n+1!}) \circ
  \hat{\tau}_n^*(\sigma_{0,n!}) \circ \tau_{n!}
\end{equation}
\end{subequations}
%
\subsection{Showing Equations \ref{eq:strict} hold}
Equation \ref{eq:strict_1} has three relations. 
All of the $\sigma_!$'s and $\delta_!$'s in Equation 
\ref{eq:strict_1} are identity maps, so it's clear that 
these relations hold.

Equation \ref{eq:strict_2} has two relations. 
To show that the first one holds, we have
\begin{align*}
\hat{\sigma}_{i,n}^*(\tau_{n+1!}) \circ \sigma_{i,n!} 
&= 
\hat{\sigma}_{i,n}^*(
  (\widehat{\delta_{0,2}\smdots\delta_{0,n+1}})^*
  (\tau_{1!})) \circ \sigma_{i,n!}
  \quad \textrm{definition of }\tau_{n+1!}\\
&= 
(\widehat{\delta_{0,2}\smdots\delta_{0,n+1}\sigma_{i,n}})^*
  (\tau_{1!}) \circ \sigma_{i,n!}
  \quad \textrm{Proposition } \ref{prop:pbs_compose}\\
&= 
(\widehat{\delta_{0,2}\smdots\delta_{0,n}})^*
  (\tau_{1!}) \circ \sigma_{i,n!}\\
&= 
\tau_{n!} \circ \sigma_{i,n!}
  \quad \textrm{definition of }\tau_{n!}\\
&= 
\tau_{n!} \circ id  
  = id \circ \tau_{n!} \\
&= 
\hat{\tau}_n^*(\sigma_{i+1,n!}) \circ \tau_{n!}.
\end{align*}
To show that the second relation holds, the 
reasoning is the same as above. We have
\begin{align*}
\hat{\delta}_{j,n}^*(\tau_{n-1!}) \circ \delta_{j,n!} 
&= 
\hat{\delta}_{j,n}^*
  ((\widehat{\delta_{0,2}\smdots\delta_{0,n-1}})^*
  (\tau_{1!})) \circ \delta_{j,n!} \\
&=
(\widehat{\delta_{0,2}\smdots\delta_{0,n-1}\delta_{j,n}})^*
  (\tau_{1!}) \circ \delta_{j,n!} \\
&=
\tau_{n!} \circ \delta_{j,n!}\\
&= 
\tau_{n!} \circ id   
  = id \circ \tau_{n!}\\
&=
\hat{\tau}_n^*(\delta_{j+1,n!}) \circ \tau_{n!}. 
\end{align*} 

Equation \ref{eq:strict_3} has one relation. 
The only map in this relation that is not 
defined to be an identity map is $\hat{\sigma}_{0,0}^*
(\tau_{1!})$. We will compute this map and 
show that it is also an identity. 
Let $(\phi_{0,1}\smdots \phi_{0,k_0}|\alpha)
\in C(A_0 \to A_0)$ (see Figure \ref{fig:phi|alpha} 
for notation). By Proposition \ref{prop:compute_pb},
\begin{align*}
C(A_0 \to A_0)
&\xrightarrow{\cong} 
\hat{\sigma}_{0,0}^*C(A_0 \to A_0 \to A_0)\\
(\phi_{0,1}\smdots \phi_{0,k_0}|\alpha)
&\mapsto
\sum \limits_{0 \leq r_0 \leq k_0}
  (\phi_{0,1}\smdots \phi_{0,r_0}) \otimes 
  (1 | \phi_{0,r_0+1}\smdots \phi_{0,k_0}|\alpha).
\end{align*}
Applying $\hat{\sigma}_{0,0}^*(\tau_{1!})$
to the righthand side, we have
\begin{align*}
\hat{\sigma}_{0,0}^*C(A_0 \to A_0 \to A_0)
&\xrightarrow{\hat{\sigma}_{0,0}^*(\tau_{1!})}
\hat{\sigma}_{0,0}^*\hat{\tau}_1^*C(A_0 \to A_0 \to A_0)\\
\sum \limits_{0 \leq r_0 \leq k_0}
  (\phi_{0,1}\smdots \phi_{0,r_0}) \otimes 
  (1 | \phi_{0,r_0+1}\smdots \phi_{0,k_0}|\alpha)
&\mapsto
\sum \limits_{0 \leq r_0 \leq s_0 \leq k_0}
  (\phi_{0,1}\smdots \phi_{0,r_0}) \otimes \\
&\phantom{{}\mapsto \sum{}}  
  (\phi_{0,r_0+1}\smdots \phi_{0,s_0}|1|
  \tau_1(1|\phi_{0,s_0+1}\smdots\phi_{0,k_0}|\alpha)).
\end{align*}
The righthand side above is equal to
\begin{align*}
&\phantom{{}={}}
\sum \limits_{0 \leq r_0 \leq s_0 \leq k_0}
  (\phi_{0,1}\smdots \phi_{0,r_0}) \otimes 
  (\phi_{0,r_0+1}\smdots \phi_{0,s_0}|1|
  \tau_1(1|\phi_{0,s_0+1}\smdots\phi_{0,k_0}|\alpha))\\
&=  
\sum \limits_{0 \leq r_0 \leq s_0 \leq k_0}
  (\phi_{0,1}\smdots \phi_{0,r_0}) \otimes 
  (\phi_{0,r_0+1}\smdots \phi_{0,s_0}|1|
  \upsilon_{0,k_0-s_0}(1|\phi_{0,s_0+1}\smdots\phi_{0,k_0}|\alpha))\\
&\phantom{{}=\sum\sum{}}  
  \quad \textrm{(see Proposition \ref{prop:c1} for }
  \upsilon_{\cdot,\cdot})\\
&=  
\sum \limits_{0 \leq r_0 \leq k_0}
  (\phi_{0,1}\smdots \phi_{0,r_0}) \otimes 
  (\phi_{0,r_0+1}\smdots \phi_{0,k_0}|1|\alpha)
  \quad \quad (\upsilon_{0,>0}=0)\\
&\in
\hat{\sigma}_{0,0}^*\hat{\tau}_1^*C(A_0 \to A_0 \to A_0).
\end{align*}
Finally, applying Proposition 
\ref{prop:compute_pb} again, we have
\begin{align*}
\hat{\sigma}_{0,0}^*\hat{\tau}_1^*C(A_0 \to A_0 \to A_0)
&\xrightarrow[\cong]{\textrm{project onto cogenerators}} 
C(A_0 \to A_0)\\
\sum \limits_{0 \leq r_0 \leq k_0}
  (\phi_{0,1}\smdots \phi_{0,r_0}) \otimes 
  (\phi_{0,r_0+1}\smdots \phi_{0,k_0}|1|\alpha)
&\mapsto
(\phi_{0,1}\smdots \phi_{0,k_0}|\alpha).
\end{align*}
So, we've shown 
$$
C(A_0 \to A_0) \cong 
\hat{\sigma}_{0,0}^*C(A_0 \to A_0 \to A_0)
\xrightarrow{\hat{\sigma}_{0,0}^*(\tau_{1!})}
\hat{\sigma}_{0,0}^*\hat{\tau}_1^*C(A_0 \to A_0 \to A_0)
\cong C(A_0 \to A_0)
$$
is the identity map.
% 
\subsection{Showing Equations \ref{eq:weak} hold}
First, we will show that Equation 
\ref{eq:weak_delta} holds. Then, we will 
show that Equation 
\ref{eq:weak_delta} implies Equation 
\ref{eq:weak_tau}, and Equation \ref{eq:weak_tau} 
implies Equation \ref{eq:weak_sigma}.

\subsubsection{Showing Equation \ref{eq:weak_delta} holds}
For $n=1$, eliminating the identity 
maps reduces Equation \ref{eq:weak_delta} to:
\begin{align*} 
\hat{\tau}_1^*(\tau_{1!}) \circ \tau_{1!} 
\simeq id.
\end{align*}
We prove the above in Appendix Proposition 
\ref{prop:c2}. (In the appendix, 
$\tau_{1!} = \Upsilon_{A_0,A_1}$, 
$\hat{\tau}_1^*(\tau_{1!}) = \Upsilon_{A_1,A_0}$, 
and the homotopy is denoted $B$.)

For $n=2$, eliminating the identity 
maps and writing $\tau_{2!}$ in terms 
of $\tau_{1!}$ reduces Equation \ref{eq:weak_delta} to:
\begin{align*} 
(\widehat{\delta_{0,2}\tau_2})^*(\tau_{1!}) \circ 
  \hat{\delta}_{0,2}^*(\tau_{1!})
\simeq \hat{\delta}_{1,2}^*(\tau_{1!}).
\end{align*}
We prove the above in Appendix Proposition 
\ref{prop:c4}. (In the appendix, 
$\hat{\delta}_{0,2}^*(\tau_{1!}) = 
\Upsilon_{A_0\bullet A_1, A_2}$, 
$(\widehat{\delta_{0,2}\tau_2})^*(\tau_{1!}) 
= \Upsilon_{A_2\bullet A_0,A_1}$, 
$\hat{\delta}_{1,2}^*(\tau_{1!}) =
\Upsilon_{A_0, A_1\bullet A_2}$, 
and the homotopy is denoted 
$\mathcal{B}$.)

For $n>2$, we reduce Equation 
\ref{eq:weak_delta} to the case when 
$n=2$. We have
\begin{align*}
\textrm{Lefthand side of Equation 
\ref{eq:weak_delta}}
&= 
\hat{\tau}_n^{*2}(\delta_{0,n!}) \circ 
  \hat{\tau}_n^*(\tau_{n!}) \circ \tau_{n!} \\  
&=  
id \circ 
  \hat{\tau}_n^*(
  (\widehat{\delta_{0,2}\smdots\delta_{0,n}})^*(\tau_{1!})) 
  \circ \tau_{n!} \\
&=   
(\widehat{\delta_{0,2}\smdots\delta_{0,n}\tau_n})^*(\tau_{1!}) 
  \circ \tau_{n!} \\
&=
(\widehat{\delta_{0,2}\tau_2\delta_{0,3}\smdots\delta_{0,n}})^*(\tau_{1!}) 
  \circ \tau_{n!} \\
&=
(\widehat{\delta_{0,2}\tau_2\delta_{0,3}\smdots\delta_{0,n}})^*(\tau_{1!}) 
  \circ (\widehat{\delta_{0,2}\smdots\delta_{0,n}\tau_n})^*(\tau_{1!}) \\
&=
(\widehat{\delta_{0,3}\smdots\delta_{0,n}})^*(
  (\widehat{\delta_{0,2}\tau_2})^*(\tau_{1!}) 
  \circ \hat{\delta}_{0,2}^*\tau_{1!}) \\ 
%
\textrm{Righthand side of Equation 
\ref{eq:weak_delta}}
&=  
\hat{\delta}_{n-1,n}^*(\tau_{n-1!}) 
  \circ \delta_{n-1,n!}\\
&=  
\hat{\delta}_{n-1,n}^*(
  (\widehat{\delta_{0,2}\smdots\delta_{0,n-1}})^*
  (\tau_{1!})) \circ id\\
&=  
(\widehat{\delta_{0,2}\smdots\delta_{0,n-1}
  \delta_{n-1,n}})^*(\tau_{1!}))\\  
&=  
(\widehat{\delta_{1,2}\delta_{0,3}\smdots\delta_{0,n}})^*
  (\tau_{1!})\\ 
&=  
(\widehat{\delta_{0,3}\smdots\delta_{0,n}})^*
  (\hat{\delta}_{1,2}^*(\tau_{1!})).
\end{align*}
So, Equation \ref{eq:weak_delta} = 
$(\widehat{\delta_{0,3}\smdots\delta_{0,n}})^*$(
Equation \ref{eq:weak_delta}, $n=2$). 
If $\mathcal{B}$ is a homotopy giving 
Equation \ref{eq:weak_delta} for $n=2$, then 
$(\widehat{\delta_{0,3}\smdots\delta_{0,n}})^*
\mathcal{B}$ is a homotopy giving Equation 
\ref{eq:weak_delta} for $n>2$.
%
\subsubsection{Showing Equation \ref{eq:weak_tau} holds}
We prove this by induction on $n$. For $n=1$, 
Equation \ref{eq:weak_tau} is the same as 
Equation \ref{eq:weak_delta}, which we 
established in the previous section. Now, 
assume that Equation \ref{eq:weak_tau} holds 
for $N=n-1$. We want to show that Equation 
\ref{eq:weak_tau} holds for $N=n$.
%
\subsubsection{Showing Equation \ref{eq:weak_sigma} holds}